added select and save

fstar/Storage.fst
@@ -1,11 +1,15 @@
 module Storage
 
-type value a =
-  | Mtst : value a
-  | Var : (v : a) -> value a
-  | Store : (st : value a) -> (k : nat) -> (v : value a) -> value a
+type value a b c =
+  | Mtst : value a b c
+  | Var : (v : a) -> value a b c
+  | Store : (st : value a b c) -> (k : either b c) -> (v : value a b c) -> value a b c
 
-let rec save #a (st : value a) (flds : list nat)  (v : value a) : value a
+let rec save #a (#b : eqtype) (#c : eqtype)  (st : value a b c) (flds : list (either b c))  (v : value a b c)
+  : Tot (value a b c) (decreases st)
   = match st, flds with
-    | Mtst, [] -> admit()
-    | _, _ -> admit()
+    | Mtst, [] -> v
+    | Mtst, k :: xs -> Store Mtst k (save Mtst xs v)
+    | Var _, _ -> v
+    | Store st x v', [] -> Store st x v'
+    | Store st k v', k' :: ys -> if k = k' then Store st k (save v ys v') else Store (save st (k' :: ys) v') k v
